

$$2\ddot{x} + 4\dot{x} + 3x = 1 \quad x(0) = 2, \quad \dot{x}(0) = 1$$

$$2[s^2 X(s) - s x(0) - \dot{x}(0)] + 4[s X(s) - x(0)] + 3X(s) = \frac{1}{s}$$

$$2(s^2 X(s) - 2s - 1) + 4(s X(s) - 2) + 3X(s) = \frac{1}{s}$$

$$X(s)(2s^2 + 4s + 3) = \frac{1}{s} + 4s + 2 + 8 = \frac{4s^2 + 10s + 1}{s}$$

$$X(s) = \frac{4s^2 + 10s + 1}{(2s^2 + 4s + 3)s} = \frac{2s^2 + 5s + \frac{1}{2}}{s(s^2 + 2s + \frac{3}{2})} = \frac{2s^2 + 5s + \frac{1}{2}}{s((s+1)^2 + \frac{1}{2})}$$

$$= \frac{A}{s} + \frac{Bs + C}{(s+1)^2 + \frac{1}{2}}$$

$$2s^2 + 5s + \frac{1}{2} = A(s^2 + 2s + \frac{3}{2}) + Bs^2 + Cs$$

MATCH COEFF'S:

$$s^2: 2 = A + B \Rightarrow B = \frac{5}{3}$$

$$s^1: 5 = 2A + C \Rightarrow C = \frac{13}{3}$$

$$s^0: \frac{1}{2} = \frac{3}{2}A \Rightarrow A = \frac{1}{3}$$

$$X(s) = \frac{\frac{1}{3}}{s} + \frac{\frac{5}{3}s + \frac{13}{3}}{(s+1)^2 + (\sqrt{\frac{1}{2}})^2} \Rightarrow \omega = \sqrt{\frac{1}{2}}$$

$$= \frac{\frac{1}{3}}{s} + \frac{\frac{5}{3}(s+1)}{(s+1)^2 + (\sqrt{\frac{1}{2}})^2} + \frac{\frac{8}{3}(\sqrt{2})(\sqrt{\frac{1}{2}})}{(s+1)^2 + (\sqrt{\frac{1}{2}})^2}$$

$$\therefore x(t) = \left(\frac{1}{3} + \frac{5}{3} e^{-t} \cos \sqrt{\frac{1}{2}} t + \frac{8\sqrt{2}}{3} e^{-t} \sin \sqrt{\frac{1}{2}} t \right) u(t)$$